transformations/Moore2MealyALT/MooreWF.v
@@ -3,11 +3,11 @@ Require Import Moore2MealyALT.Moore Moore2MealyALT.MooreSemantics.
 Import String.
 Import Id.
 
-Definition unique_names (m:Moore.M) := 
+Definition unique_ids (m:Moore.M) := 
   forall e1 e2,
     List.In (StateElement e1) m.(Model.modelElements) ->
     List.In (StateElement e2) m.(Model.modelElements) ->
-    e1.(State_name) = e2.(State_name) ->
+    e1.(State_id) = e2.(State_id) ->
     e1 = e2.
 
 Lemma In_state : forall (m:Moore.M) e,
@@ -50,10 +50,10 @@ Qed.
 
 
 Lemma discr  (m : M) : 
-  unique_names m ->
+  unique_ids m ->
   forall (i : NodeId),
     ListUtils.discriminating_predicate
-      (fun x : State_t => NodeId_beq i (State_name x) = true)
+      (fun x : State_t => NodeId_beq i (State_id x) = true)
       (OptionListUtils.lift_list (get_E_data State_K)
          (Model.modelElements m)).
 Proof.
@@ -69,11 +69,11 @@ Qed.
 
 Lemma in_find : 
   forall m n e,
-    unique_names m ->
+    unique_ids m ->
     List.In (StateElement e) m.(Model.modelElements) ->
-    e.(State_name) = n ->
+    e.(State_id) = n ->
     OptionListUtils.find_lift (get_E_data State_K)
-           (fun s : State_t => (NodeId_beq n  s.(State_name))%string)
+           (fun s : State_t => (NodeId_beq n  s.(State_id))%string)
            m.(Model.modelElements) = 
          Some e.
 Proof.
@@ -86,10 +86,10 @@ Qed.
 
 
 
-Lemma getTransition_sourcet_some (s:State_t) t (m:Moore.M) :
-  unique_names m ->
+Lemma getTransition_source_some (s:State_t) t (m:Moore.M) :
+  unique_ids m ->
   List.In (StateElement s) m.(Model.modelElements) ->
-  State_name s = t.(Transition_source) ->
+  State_id s = t.(Transition_source) ->
   getTransition_source m t = Some s. 
 Proof.
   intros WF H1 H2.
@@ -101,9 +101,9 @@ Proof.
 Qed.
  
 Lemma getTransition_target_some (s:State_t) t (m:Moore.M) :
-  unique_names m ->
+  unique_ids m ->
   List.In (StateElement s) m.(Model.modelElements) ->
-  State_name s = t.(Transition_dest) ->
+  State_id s = t.(Transition_dest) ->
   getTransition_target m t = Some s. 
 Proof.
   intros WF H1 H2.
